CBPV/Normalization.lean
@@ -6,16 +6,15 @@ import CBPV.NormalAcc
   via soundness of typing wrt semantic typing
 --------------------------------------------*-/
 
-theorem normalization' {Γ} :
-  (∀ {v : Val} {A}, Γ ⊢ v ∶ A → SNVal v) ∧
-  (∀ {m : Com} {B}, Γ ⊢ m ∶ B → SNCom m) := by
-  let ⟨soundVal, soundCom⟩ := @soundness Γ
-  refine ⟨λ h ↦ ?val, λ h ↦ ?com⟩
-  case val =>
+joint {Γ : Ctxt}
+  theorem ValWt.normalization' {v : Val} {A} (h : Γ ⊢ v ∶ A) : SNVal v
+  theorem ComWt.normalization' {m : Com} {B} (h : Γ ⊢ m ∶ B) : SNCom m
+by
+  case ValWt =>
     let ⟨_, hA, pv⟩ := soundVal _ _ h _ semCtxtVar
     rw [substValId] at pv
     exact hA.snVal pv
-  case com =>
+  case ComWt =>
     let ⟨_, hB, pm⟩ := soundCom _ _ h _ semCtxtVar
     rw [substComId] at pm
     exact hB.snCom pm
@@ -28,29 +27,29 @@ theorem normalization' {Γ} :
 theorem NeCom.ne {m} (snem : SNeCom m) : NeCom m := by
   mutual_induction snem <;> assumption
 
-theorem SN_soundness :
-  (∀ {m}, SNeCom m → StepCom.SN m) ∧
-  (∀ {v}, SNVal  v → StepVal.SN v) ∧
-  (∀ {m}, SNCom  m → StepCom.SN m) ∧
-  (∀ {m n : Com}, m ⤳ n → m ⤳ⁿ n) := by
-  refine ⟨λ sne ↦ ?snecom, λ sn ↦ ?snval, λ sn ↦ ?sncom, λ r ↦ ?srcom⟩
+joint
+  theorem SNeCom.SN_soundness {m} (sne : SNeCom m) : StepCom.SN m
+  theorem SNVal.SN_soundness {v} (sn : SNVal v) : StepVal.SN v
+  theorem SNCom.SN_soundness {m} (sn : SNCom  m) : StepCom.SN m
+  theorem Sr.SN_soundness {m n : Com} (r : m ⤳ n) : m ⤳ⁿ n
+by
   mutual_induction sne, sn, sn, r
-  case snecom.force snv => exact .force snv
-  case snecom.app snem _ snm snv => exact .app (.ne snem) snm snv
-  case snecom.letin snem _ snm snn => exact .letin (.ne snem) snm snn
-  case snecom.case snv _ _ snm snn => exact .case snv snm snn
-  case snecom.fst snem snm => exact .fst (.ne snem) snm
-  case snecom.snd snem snm => exact .snd (.ne snem) snm
-  case snval.var => constructor; intro _ r; cases r
-  case snval.unit => constructor; intro _ r; cases r
-  case snval.inl ih => exact .inl ih
-  case snval.inr ih => exact .inr ih
-  case snval.thunk ih => exact .thunk ih
-  case sncom.lam ih => exact .lam ih
-  case sncom.ret ih => exact .ret ih
-  case sncom.prod ihm ihn => exact .prod ihm ihn
-  case sncom.ne => assumption
-  case sncom.red r ih => exact r.closure ih
+  case force snv => exact .force snv
+  case app snem _ snm snv => exact .app (.ne snem) snm snv
+  case letin snem _ snm snn => exact .letin (.ne snem) snm snn
+  case case snv _ _ snm snn => exact .case snv snm snn
+  case fst snem snm => exact .fst (.ne snem) snm
+  case snd snem snm => exact .snd (.ne snem) snm
+  case var => constructor; intro _ r; cases r
+  case unit => constructor; intro _ r; cases r
+  case inl ih => exact .inl ih
+  case inr ih => exact .inr ih
+  case thunk ih => exact .thunk ih
+  case lam ih => exact .lam ih
+  case ret ih => exact .ret ih
+  case prod ihm ihn => exact .prod ihm ihn
+  case ne => assumption
+  case red r ih => exact r.closure ih
   all_goals constructor <;> assumption
 
 /-*------------------------------------------
@@ -58,7 +57,7 @@ theorem SN_soundness :
 ------------------------------------------*-/
 
 theorem ValWt.normalization {Γ} {v : Val} {A} (h : Γ ⊢ v ∶ A) : StepVal.SN v :=
-  SN_soundness.right.left (normalization'.left h)
+  h.normalization'.SN_soundness
 
 theorem ComWt.normalization {Γ} {m : Com} {B} (h : Γ ⊢ m ∶ B) : StepCom.SN m :=
-  SN_soundness.right.right.left (normalization'.right h)
+  h.normalization'.SN_soundness
